Port LDRF-SC

src/ldrfsc/SCStep.v
@@ -11,127 +11,120 @@ From PromisingLib Require Import DataStructure.
 From PromisingLib Require Import DenseOrder.
 From PromisingLib Require Import Loc.
 From PromisingLib Require Import Language.
-From PromisingLib Require Import Event.
 
+From PromisingLib Require Import Event.
 Require Import Time.
 Require Import View.
-Require Import BoolMap.
-Require Import Promises.
 Require Import Cell.
 Require Import Memory.
-Require Import TView.
 Require Import Global.
+Require Import TView.
 Require Import Local.
 Require Import Thread.
 Require Import Configuration.
+Require Import BoolMap.
+Require Import Promises.
+
+Require Import OrdStep.
 
 Set Implicit Arguments.
 
 
-Module OrdLocal.
-  Section OrdLocal.
-    Variable L: Loc.t -> bool.
-    Variable ordcr: Ordering.t.
-    Variable ordcw: Ordering.t.
 
-    Variant read_step (lc1:Local.t) (gl1:Global.t) (loc:Loc.t) (to:Time.t) (val:Const.t) (released:option View.t) (ord:Ordering.t) (lc2:Local.t): Prop :=
+
+(** L-SC machine **)
+Module SCLocal.
+  Section SCLocal.
+    Variable L: Loc.t -> bool.
+
+    Definition non_maximal (lc: Local.t) (mem: Memory.t) (loc: Loc.t): Prop :=
+      exists to from msg,
+        (<<GET: Memory.get loc to mem = Some (from, msg)>>) /\
+        (<<NRESERVE: msg <> Message.reserve>>) /\
+        (<<TS: Time.lt ((TView.cur (Local.tview lc)).(View.rlx) loc) to>>)
+    .
+
+    Inductive read_step (lc1:Local.t) (gl1:Global.t) (loc:Loc.t) (to:Time.t) (val:Const.t) (released:option View.t) (ord:Ordering.t) (lc2:Local.t): Prop :=
     | read_step_intro
         ord'
-        (ORD: ord' = if L loc then Ordering.join ord ordcr else ord)
+        (ORD: ord' = if L loc then Ordering.join ord Ordering.acqrel else ord)
         (STEP: Local.read_step lc1 gl1 loc to val released ord' lc2)
+        (MAXIMAL: forall (LOC: L loc)
+                         from' to' val' released' na
+                         (GET: Memory.get loc to' gl1.(Global.memory) = Some (from', Message.message val' released' na)),
+            Time.le to' to)
     .
     Hint Constructors read_step: core.
 
-    Variant write_step (lc1:Local.t) (gl1:Global.t)
+    Inductive write_step (lc1:Local.t) (gl1:Global.t)
               (loc:Loc.t) (from to:Time.t)
               (val:Const.t) (releasedm released:option View.t) (ord:Ordering.t)
               (lc2:Local.t) (gl2:Global.t): Prop :=
     | write_step_intro
         ord'
-        (ORD: ord' = if L loc then Ordering.join ord ordcw else ord)
+        (ORD: ord' = if L loc then Ordering.join ord Ordering.acqrel else ord)
         (STEP: Local.write_step lc1 gl1 loc from to val releasedm released ord' lc2 gl2)
+        (MAXIMAL: forall (LOC: L loc)
+                         from' to' val' released' na
+                         (GET: Memory.get loc to' gl1.(Global.memory) = Some (from', Message.message val' released' na)),
+            Time.lt to' to)
     .
     Hint Constructors write_step: core.
 
-    Variant racy_read_step (lc1:Local.t) (gl1:Global.t) (loc:Loc.t) (to:option Time.t) (val:Const.t) (ord:Ordering.t): Prop :=
-    | racy_read_step_intro
-        ord'
-        (ORD: ord' = if L loc then Ordering.join ord ordcr else ord)
-        (STEP: Local.racy_read_step lc1 gl1 loc to val ord')
-    .
-    Hint Constructors racy_read_step: core.
-
-    Variant racy_write_step (lc1:Local.t) (gl1:Global.t) (loc:Loc.t) (to:option Time.t) (ord:Ordering.t): Prop :=
-    | racy_write_step_intro
-        ord'
-        (ORD: ord' = if L loc then Ordering.join ord ordcw else ord)
-        (STEP: Local.racy_write_step lc1 gl1 loc to ord')
-    .
-    Hint Constructors racy_write_step: core.
-
     Variant program_step:
-      forall (e:ThreadEvent.t) (lc1:Local.t) (gl1:Global.t) (lc2:Local.t) (gl2:Global.t), Prop :=
-    | step_silent
-        lc1 gl1:
+      forall (e: ThreadEvent.t) (lc1: Local.t) (gl1: Global.t) (lc2: Local.t) (gl2: Global.t), Prop :=
+      | program_step_silent
+          lc1 gl1:
         program_step ThreadEvent.silent lc1 gl1 lc1 gl1
-    | step_read
-        lc1 gl1
-        loc ts val released ord lc2
-        (LOCAL: read_step lc1 gl1 loc ts val released ord lc2):
-        program_step (ThreadEvent.read loc ts val released ord) lc1 gl1 lc2 gl1
-    | step_write
-        lc1 gl1
-        loc from to val released ord lc2 gl2
-        (LOCAL: write_step lc1 gl1 loc from to val None released ord lc2 gl2):
+      | program_step_read
+          lc1 gl1
+          loc to val released ord lc2
+          (LOCAL: read_step lc1 gl1 loc to val released ord lc2):
+        program_step (ThreadEvent.read loc to val released ord) lc1 gl1 lc2 gl1
+      | program_step_write
+          lc1 gl1
+          loc from to val released ord lc2 gl2
+          (LOCAL: write_step lc1 gl1 loc from to val None released ord lc2 gl2):
         program_step (ThreadEvent.write loc from to val released ord) lc1 gl1 lc2 gl2
-    | step_update
-        lc1 gl1
-        loc ordr ordw
-        tsr valr releasedr releasedw lc2
-        tsw valw lc3 gl3
-        (LOCAL1: read_step lc1 gl1 loc tsr valr releasedr ordr lc2)
-        (LOCAL2: write_step lc2 gl1 loc tsr tsw valw releasedr releasedw ordw lc3 gl3):
+      | program_step_update
+          lc1 gl1
+          loc ordr ordw
+          tsr valr releasedr releasedw lc2
+          tsw valw lc3 gl3
+          (LOCAL1: read_step lc1 gl1 loc tsr valr releasedr ordr lc2)
+          (LOCAL2: write_step lc2 gl1 loc tsr tsw valw releasedr releasedw ordw lc3 gl3):
         program_step (ThreadEvent.update loc tsr tsw valr valw releasedr releasedw ordr ordw)
                      lc1 gl1 lc3 gl3
-    | step_fence
-        lc1 gl1
-        ordr ordw lc2 gl2
-        (LOCAL: Local.fence_step lc1 gl1 ordr ordw lc2 gl2):
+      | program_step_fence
+          lc1 gl1
+          ordr ordw lc2 gl2
+          (LOCAL: Local.fence_step lc1 gl1 ordr ordw lc2 gl2):
         program_step (ThreadEvent.fence ordr ordw) lc1 gl1 lc2 gl2
-    | step_syscall
-        lc1 gl1
-        e lc2 gl2
-        (LOCAL: Local.fence_step lc1 gl1 Ordering.seqcst Ordering.seqcst lc2 gl2):
+      | program_step_syscall
+          lc1 gl1
+          e lc2 gl2
+          (LOCAL: Local.fence_step lc1 gl1 Ordering.seqcst Ordering.seqcst lc2 gl2):
         program_step (ThreadEvent.syscall e) lc1 gl1 lc2 gl2
-    | step_failure
-        lc1 gl1
-        (LOCAL: Local.failure_step lc1):
-      program_step ThreadEvent.failure lc1 gl1 lc1 gl1
-    | step_racy_read
-        lc1 gl1
-        loc to val ord
-        (LOC: ~ L loc)
-        (LOCAL: Local.racy_read_step lc1 gl1 loc to val ord):
-      program_step (ThreadEvent.racy_read loc to val ord) lc1 gl1 lc1 gl1
-    | step_racy_write
-        lc1 gl1
-        loc to val ord
-        (LOC: ~ L loc)
-        (LOCAL: Local.racy_write_step lc1 gl1 loc to ord):
-      program_step (ThreadEvent.racy_write loc to val ord) lc1 gl1 lc1 gl1
-    | step_racy_update
-        lc1 gl1
-        loc to valr valw ordr ordw
-        (LOC: ~ L loc)
-        (LOCAL: Local.racy_update_step lc1 gl1 loc to ordr ordw):
-      program_step (ThreadEvent.racy_update loc to valr valw ordr ordw) lc1 gl1 lc1 gl1
-    | step_na_update
-        lc1 gl1
-        loc valr valw ordr ordw
-        (NA: Ordering.le ordr Ordering.na \/ Ordering.le ordw Ordering.na):
-      program_step (ThreadEvent.racy_update loc None valr valw ordr ordw) lc1 gl1 lc1 gl1
+      | program_step_failure
+          lc1 gl1
+          (LOCAL: Local.failure_step lc1):
+        program_step ThreadEvent.failure lc1 gl1 lc1 gl1
+      | program_step_racy_read
+          lc1 gl1
+          loc to val ord
+          (LOCAL: Local.racy_read_step lc1 gl1 loc to val ord):
+        program_step (ThreadEvent.racy_read loc to val ord) lc1 gl1 lc1 gl1
+      | program_step_racy_write
+          lc1 gl1
+          loc to val ord
+          (LOCAL: Local.racy_write_step lc1 gl1 loc to ord):
+        program_step (ThreadEvent.racy_write loc to val ord) lc1 gl1 lc1 gl1
+      | program_step_racy_update
+          lc1 gl1
+          loc to valr valw ordr ordw
+          (LOCAL: Local.racy_update_step lc1 gl1 loc to ordr ordw):
+        program_step (ThreadEvent.racy_update loc to valr valw ordr ordw) lc1 gl1 lc1 gl1
     .
-    Hint Constructors program_step: core.
 
 
     (* step_future *)
@@ -139,11 +132,11 @@ Module OrdLocal.
     Lemma program_step_future
           e lc1 gl1 lc2 gl2
           (STEP: program_step e lc1 gl1 lc2 gl2)
-          (LC_WF1: Local.wf lc1 gl1)
-          (GL_WF1: Global.wf gl1):
-      <<LC_WF2: Local.wf lc2 gl2>> /\
-      <<GL_WF2: Global.wf gl2>> /\
-      <<TVIEW_FUTURE: TView.le (Local.tview lc1) (Local.tview lc2)>> /\
+          (WF1: Local.wf lc1 gl1)
+          (GL1: Global.wf gl1):
+      <<WF2: Local.wf lc2 gl2>> /\
+      <<GL2: Global.wf gl2>> /\
+      <<TVIEW_FUTURE: TView.le lc1.(Local.tview) lc2.(Local.tview)>> /\
       <<GL_FUTURE: Global.future gl1 gl2>>.
     Proof.
       inv STEP.
@@ -152,15 +145,14 @@ Module OrdLocal.
         exploit Local.read_step_future; eauto. i. des.
         esplits; eauto; try refl.
       - inv LOCAL.
-        exploit Local.write_step_future; eauto;
-          (try by econs); (try apply Time.bot_spec). i. des.
+        exploit Local.write_step_future; eauto; try by econs.
+        { ss. eapply Time.bot_spec. }
+        i. des.
         esplits; eauto; try refl.
       - inv LOCAL1. inv LOCAL2.
         exploit Local.read_step_future; eauto. i. des.
         exploit Local.write_step_future; eauto; try by econs.
-        { etrans; eauto. inv STEP0.
-          econs. eauto using Memory.add_ts.
-        }
+        { etrans; eauto. inv STEP0. inv WRITE. inv ADD. left. auto. }
         i. des.
         esplits; eauto. etrans; eauto.
       - exploit Local.fence_step_future; eauto.
@@ -169,18 +161,6 @@ Module OrdLocal.
       - esplits; eauto; try refl.
       - esplits; eauto; try refl.
       - esplits; eauto; try refl.
-      - esplits; eauto; try refl.
-    Qed.
-
-    Lemma program_step_inhabited
-          e lc1 gl1 lc2 gl2
-          (STEP: program_step e lc1 gl1 lc2 gl2)
-          (INHABITED1: Memory.inhabited gl1.(Global.memory)):
-      <<INHABITED2: Memory.inhabited gl2.(Global.memory)>>.
-    Proof.
-      inv STEP; try inv LOCAL; ss.
-      - inv STEP. eapply Memory.add_inhabited; eauto.
-      - inv LOCAL2. inv STEP. eapply Memory.add_inhabited; eauto.
     Qed.
 
 
@@ -189,12 +169,12 @@ Module OrdLocal.
     Lemma program_step_disjoint
           e lc1 gl1 lc2 gl2 lc
           (STEP: program_step e lc1 gl1 lc2 gl2)
-          (LC_WF1: Local.wf lc1 gl1)
-          (GL_WF1: Global.wf gl1)
+          (WF1: Local.wf lc1 gl1)
+          (GL1: Global.wf gl1)
           (DISJOINT1: Local.disjoint lc1 lc)
-          (LC_WF: Local.wf lc gl1):
+          (WF: Local.wf lc gl1):
       <<DISJOINT2: Local.disjoint lc2 lc>> /\
-      <<LC_WF: Local.wf lc gl2>>.
+      <<WF: Local.wf lc gl2>>.
     Proof.
       inv STEP.
       - esplits; eauto.
@@ -206,7 +186,6 @@ Module OrdLocal.
         exploit Local.write_step_disjoint; eauto.
       - exploit Local.fence_step_disjoint; eauto.
       - exploit Local.fence_step_disjoint; eauto.
-      - esplits; eauto.
       - esplits; eauto.
       - esplits; eauto.
       - esplits; eauto.
@@ -281,80 +260,27 @@ Module OrdLocal.
       inv STEP; try inv LOCAL; ss; try inv STEP; ss.
       inv LOCAL1. inv LOCAL2. inv STEP. inv STEP0. ss.
     Qed.
-
-    Lemma ordc_na
-          ordc ord loc
-          (ORDC: Ordering.le ordc Ordering.na):
-      (if L loc then Ordering.join ord ordc else ord) = ord.
-    Proof.
-      condtac; ss.
-      destruct ordc, ord; ss.
-    Qed.
-
-    (* Lemma write_step_le *)
-    (*       lc1 sc1 mem1 loc from to val releasedm released ord lc2 sc2 mem2 kind *)
-    (*       ordc' *)
-    (*       (STEP: write_step lc1 sc1 mem1 loc from to val releasedm released *)
-    (*                         (if L loc then Ordering.join ord ordc' else ord) lc2 sc2 mem2 kind) *)
-    (*       (ORDC: Ordering.le ordc' ordcw): *)
-    (*   write_step lc1 sc1 mem1 loc from to val releasedm released ord lc2 sc2 mem2 kind. *)
-    (* Proof. *)
-    (*   econs; eauto. *)
-    (*   inv STEP. condtac; ss. *)
-    (*   replace (Ordering.join ord ordcw) with *)
-    (*       (Ordering.join (Ordering.join ord ordc') ordcw); ss. *)
-    (*   destruct ord, ordcw, ordc'; ss. *)
-    (* Qed. *)
-
-    Lemma racy_write_step_le
-          lc1 mem1 loc to ord
-          ordc'
-          (STEP: racy_write_step lc1 mem1 loc to (if L loc then Ordering.join ord ordc' else ord))
-          (ORDC: Ordering.le ordc' ordcw):
-      racy_write_step lc1 mem1 loc to ord.
-    Proof.
-      inv STEP. econs; eauto. condtac; ss.
-      replace (Ordering.join ord ordcw) with
-          (Ordering.join (Ordering.join ord ordc') ordcw); ss.
-      destruct ord, ordcw, ordc'; ss.
-    Qed.
-  End OrdLocal.
-End OrdLocal.
+  End SCLocal.
+End SCLocal.
 
 
-Module OrdThread.
-  Section OrdThread.
+Module SCThread.
+  Section SCThread.
     Variable lang: language.
     Variable L: Loc.t -> bool.
-    Variable ordcr: Ordering.t.
-    Variable ordcw: Ordering.t.
 
-    Variant step (e:ThreadEvent.t): forall (e1 e2:Thread.t lang), Prop :=
+    Inductive step (e:ThreadEvent.t): forall (e1 e2:Thread.t lang), Prop :=
     | step_intro
         st1 lc1 gl1
         st2 lc2 gl2
         (STATE: (Language.step lang) (ThreadEvent.get_program_event e) st1 st2)
-        (LOCAL: OrdLocal.program_step L ordcr ordcw e lc1 gl1 lc2 gl2):
+        (LOCAL: SCLocal.program_step L e lc1 gl1 lc2 gl2):
         step e (Thread.mk lang st1 lc1 gl1) (Thread.mk lang st2 lc2 gl2)
     .
     Hint Constructors step: core.
 
-    Definition tau_step := tau step.
-    Hint Unfold tau_step: core.
-
     Definition all_step := union step.
     Hint Unfold all_step: core.
-
-    Variant opt_step: forall (e: ThreadEvent.t) (e1 e2: Thread.t lang), Prop :=
-    | step_none
-        e:
-        opt_step ThreadEvent.silent e e
-    | step_some
-        e e1 e2
-        (STEP: step e e1 e2):
-        opt_step e e1 e2
-    .
-    Hint Constructors opt_step: core.
 
 
     (* future *)
@@ -369,7 +295,24 @@ Module OrdThread.
       <<TVIEW_FUTURE: TView.le (Local.tview (Thread.local e1)) (Local.tview (Thread.local e2))>> /\
       <<GL_FUTURE: Global.future (Thread.global e1) (Thread.global e2)>>.
     Proof.
-      inv STEP. ss. eapply OrdLocal.program_step_future; eauto.
+      inv STEP. ss. eapply SCLocal.program_step_future; eauto.
+    Qed.
+
+    Lemma rtc_all_step_future
+          e1 e2
+          (STEPS: rtc all_step e1 e2)
+          (LC_WF1: Local.wf (Thread.local e1) (Thread.global e1))
+          (GL_WF1: Global.wf (Thread.global e1)):
+      <<LC_WF2: Local.wf (Thread.local e2) (Thread.global e2)>> /\
+      <<GL_WF2: Global.wf (Thread.global e2)>> /\
+      <<TVIEW_FUTURE: TView.le (Local.tview (Thread.local e1)) (Local.tview (Thread.local e2))>> /\
+      <<GL_FUTURE: Global.future (Thread.global e1) (Thread.global e2)>>.
+    Proof.
+      revert LC_WF1 GL_WF1. induction STEPS; i.
+      - esplits; eauto; refl.
+      - inv H. inv USTEP. exploit step_future; eauto. i. des.
+        exploit IHSTEPS; eauto. i. des.
+        esplits; eauto; etrans; eauto.
     Qed.
 
 
@@ -386,7 +329,7 @@ Module OrdThread.
       <<LC_WF: Local.wf lc (Thread.global e2)>>.
     Proof.
       inv STEP.
-      eapply OrdLocal.program_step_disjoint; eauto.
+      eapply SCLocal.program_step_disjoint; eauto.
     Qed.
 
 
@@ -399,7 +342,7 @@ Module OrdThread.
       BoolMap.le (Global.promises (Thread.global th2)) (Global.promises (Thread.global th1)).
     Proof.
       inv STEP. s.
-      eapply OrdLocal.program_step_promises; eauto.
+      eapply SCLocal.program_step_promises; eauto.
     Qed.
 
     Lemma step_promises_minus
@@ -409,35 +352,26 @@ Module OrdThread.
       BoolMap.minus (Global.promises (Thread.global th2)) (Local.promises (Thread.local th2)).
     Proof.
       inv STEP; s.
-      eapply OrdLocal.program_step_promises_minus; eauto.
+      eapply SCLocal.program_step_promises_minus; eauto.
     Qed.
-  End OrdThread.
-End OrdThread.
+  End SCThread.
+End SCThread.
 
 
-Module OrdConfiguration.
-  Section OrdConfiguration.
+Module SCConfiguration.
+  Section SCConfiguration.
     Variable L: Loc.t -> bool.
-    Variable ordcr: Ordering.t.
-    Variable ordcw: Ordering.t.
 
     Variant estep: forall (e: ThreadEvent.t) (tid: Ident.t) (c1 c2: Configuration.t), Prop :=
     | estep_intro
         e tid c1 lang st1 lc1 st2 lc2 gl2
         (TID: IdentMap.find tid (Configuration.threads c1) = Some (existT _ lang st1, lc1))
-        (STEP: OrdThread.step L ordcr ordcw e
-                              (Thread.mk _ st1 lc1 (Configuration.global c1))
-                              (Thread.mk _ st2 lc2 gl2)):
-        estep e tid c1 (Configuration.mk (IdentMap.add tid (existT _ _ st2, lc2) (Configuration.threads c1)) gl2)
+        (STEP: SCThread.step L e
+                             (Thread.mk _ st1 lc1 (Configuration.global c1))
+                             (Thread.mk _ st2 lc2 gl2)):
+      estep e tid c1 (Configuration.mk (IdentMap.add tid (existT _ _ st2, lc2) (Configuration.threads c1)) gl2)
     .
     Hint Constructors estep: core.
-
-    Variant all_step (c1 c2: Configuration.t): Prop :=
-    | all_step_intro
-        e tid
-        (STEP: estep e tid c1 c2)
-    .
-    Hint Constructors all_step: core.
 
     Variant step: forall (e: MachineEvent.t) (tid: Ident.t) (c1 c2: Configuration.t), Prop :=
     | step_instro
@@ -447,6 +381,12 @@ Module OrdConfiguration.
     .
     Hint Constructors step: core.
 
+    Variant all_step (c1 c2: Configuration.t): Prop :=
+    | all_step_intro
+        e tid
+        (STEP: estep e tid c1 c2)
+    .
+    Hint Constructors all_step: core.
 
     Lemma estep_future
           e tid c1 c2
@@ -457,25 +397,25 @@ Module OrdConfiguration.
     Proof.
       inv WF1. inv WF. inv STEP; s.
       exploit THREADS; ss; eauto. i.
-      exploit OrdThread.step_future; eauto. s. i. des.
+      exploit SCThread.step_future; eauto. s. i. des.
       splits; eauto.
       econs; ss. econs.
       - i. Configuration.simplify.
         + exploit THREADS; try apply TH1; eauto. i. des.
-          exploit OrdThread.step_disjoint; eauto. s. i. des.
+          exploit SCThread.step_disjoint; eauto. s. i. des.
           symmetry. auto.
         + exploit THREADS; try apply TH2; eauto. i. des.
-          exploit OrdThread.step_disjoint; eauto. i. des.
+          exploit SCThread.step_disjoint; eauto. i. des.
           auto.
         + eapply DISJOINT; [|eauto|eauto]. auto.
       - i. Configuration.simplify.
         exploit THREADS; try apply TH; eauto. i.
-        exploit OrdThread.step_disjoint; eauto. s. i. des.
+        exploit SCThread.step_disjoint; eauto. s. i. des.
         auto.
       - i. destruct (Local.promises lc2 loc) eqn:LGET.
         + exists tid, lang, st2, lc2. splits; ss.
           rewrite IdentMap.Facts.add_o. condtac; ss.
-        + exploit OrdThread.step_promises_minus; try exact STEP0. s. i.
+        + exploit SCThread.step_promises_minus; try exact STEP0. s. i.
           eapply equal_f in x1.
           revert x1. unfold BoolMap.minus. rewrite GET, LGET. s. i.
           destruct (Global.promises (Configuration.global c1) loc) eqn:GET1; ss.
@@ -502,7 +442,7 @@ Module OrdConfiguration.
       <<WF2: Configuration.wf c2>> /\
       <<GL_FUTURE: Global.future (Configuration.global c1) (Configuration.global c2)>>.
     Proof.
-      inv STEP. eauto using estep_future.
+      inv STEP. eapply step_future; eauto.
     Qed.
 
     Lemma rtc_all_step_future
@@ -513,10 +453,57 @@ Module OrdConfiguration.
       <<GL_FUTURE: Global.future (Configuration.global c1) (Configuration.global c2)>>.
     Proof.
       revert WF1. induction STEPS; i.
-      { esplits; eauto. refl. }
-      { hexploit all_step_future; eauto. i. des.
-        hexploit IHSTEPS; eauto. i. des. esplits; eauto. etrans; eauto.
+      { splits; auto. refl. }
+      { hexploit all_step_future; eauto.
+        i. des. hexploit IHSTEPS; eauto. i. des. splits; eauto. etrans; eauto.
       }
     Qed.
-  End OrdConfiguration.
-End OrdConfiguration.
+  End SCConfiguration.
+End SCConfiguration.
+
+
+Definition is_accessing (e:ProgramEvent.t): option Loc.t :=
+  match e with
+  | ProgramEvent.read loc _ _ => Some loc
+  | ProgramEvent.write loc _ _ => Some loc
+  | ProgramEvent.update loc _ _ _ _ => Some loc
+  | _ => None
+  end.
+
+
+(** L-SC race **)
+Module SCRace.
+  Section SCRace.
+    Variable L: Loc.t -> bool.
+
+    Definition race lang (th: Thread.t lang): Prop :=
+      exists e st' loc,
+        (<<STEP: Language.step _ e (Thread.state th) st'>>) /\
+        (<<ACCESS: is_accessing e = (Some loc)>>) /\
+        (<<LOC: L loc>>) /\
+        (<<MAXIMAL: SCLocal.non_maximal th.(Thread.local) th.(Thread.global).(Global.memory) loc>>).
+
+    Definition race_steps (c: Configuration.t) (tid: Ident.t): Prop :=
+      exists lang st1 lc1,
+        (<<TID: IdentMap.find tid (Configuration.threads c) = Some (existT _ lang st1, lc1)>>) /\
+        (<<SCRACE: race (Thread.mk _ st1 lc1 c.(Configuration.global))>>).
+
+    Definition racefree (c: Configuration.t): Prop :=
+      forall tid c2
+             (STEPS: rtc (SCConfiguration.all_step L) c c2),
+        ~ race_steps c2 tid.
+
+    Definition racefree_syn (syn: Threads.syntax): Prop :=
+      racefree (Configuration.init syn).
+
+    Lemma step_racefree
+          e tid c1 c2
+          (RACEFREE: racefree c1)
+          (STEP: SCConfiguration.step L e tid c1 c2):
+      racefree c2.
+    Proof.
+      ii. eapply RACEFREE; cycle 1; eauto.
+      econs 2; eauto. inv STEP. econs; eauto.
+    Qed.
+  End SCRace.
+End SCRace.
