src/ldrfsc/LocalDRFSC.v
@@ -1,0 +1,263 @@
+Require Import Lia.
+Require Import Bool.
+Require Import RelationClasses.
+
+From sflib Require Import sflib.
+From Paco Require Import paco.
+
+From PromisingLib Require Import Axioms.
+From PromisingLib Require Import Basic.
+From PromisingLib Require Import DataStructure.
+From PromisingLib Require Import DenseOrder.
+From PromisingLib Require Import Loc.
+From PromisingLib Require Import Language.
+
+From PromisingLib Require Import Event.
+Require Import Time.
+Require Import View.
+Require Import Cell.
+Require Import Memory.
+Require Import TView.
+Require Import Local.
+Require Import Thread.
+Require Import Configuration.
+Require Import Behavior.
+Require Import Global.
+
+Require Import OrdStep.
+Require Import RARace.
+Require Import SCStep.
+Require Import Stable.
+Require Import PFConfiguration.
+
+Require Import LocalDRFRA.
+
+Section SIM.
+
+  Variable L: Loc.t -> bool.
+
+  Lemma ra_thread_step_sc_thread_step_or_race lang
+        (th0 th1: Thread.t lang) e
+        (STEP: OrdThread.step L Ordering.acqrel Ordering.acqrel e th0 th1)
+    :
+      (<<STEP: SCThread.step L e th0 th1>>) \/
+      (<<RACE: SCRace.race L th0>>).
+  Proof.
+    destruct (classic (SCRace.race L th0)) as [RACE|RACE]; auto.
+    left. inv STEP. econs; eauto. inv LOCAL; ss.
+    - econs; eauto.
+    - inv LOCAL0. econs; eauto. econs; eauto.
+      i. destruct (Time.le_lt_dec to' ts); auto. exfalso. eapply RACE.
+      unfold SCRace.race, SCLocal.non_maximal. esplits; eauto; ss.
+      inv STEP. inv READABLE. eapply TimeFacts.le_lt_lt; eauto.
+      eapply RLX. des_ifs. etrans; [|eapply Ordering.join_r]. auto.
+    - inv LOCAL0. econs; eauto. econs; eauto.
+      i. destruct (Time.le_lt_dec to to'); auto. exfalso. eapply RACE.
+      unfold SCRace.race, SCLocal.non_maximal. esplits; eauto; ss.
+      inv STEP. inv WRITABLE. eapply TimeFacts.lt_le_lt; eauto.
+    - inv LOCAL1. inv LOCAL2. econs; eauto.
+      + econs; eauto.
+        i. destruct (Time.le_lt_dec to' tsr); auto. exfalso. eapply RACE.
+        unfold SCRace.race, SCLocal.non_maximal. esplits; eauto; ss.
+        inv STEP. inv READABLE. eapply TimeFacts.le_lt_lt; eauto.
+        eapply RLX. des_ifs. etrans; [|eapply Ordering.join_r]. auto.
+      + econs; eauto.
+        i. destruct (Time.le_lt_dec tsw to'); auto. exfalso. eapply RACE.
+        unfold SCRace.race, SCLocal.non_maximal. esplits; eauto; ss.
+        inv STEP0. inv WRITABLE. eapply TimeFacts.lt_le_lt; eauto.
+        eapply TimeFacts.le_lt_lt; eauto. inv STEP. ss.
+        etrans; [|eapply Time.join_l]. eapply Time.join_l.
+    - econs; eauto.
+    - econs; eauto.
+    - econs; eauto.
+    - inv LOCAL0.
+      { econs. econs; eauto. }
+    - econs; eauto.
+    - econs; eauto.
+    - econs; eauto. des.
+      { econs 1; eauto. }
+      { econs 2; eauto. }
+  Qed.
+
+  Lemma ra_thread_all_steps_sc_thread_all_steps_or_race lang
+        (th0 th1: Thread.t lang)
+        (STEPS: rtc (OrdThread.all_step L Ordering.acqrel Ordering.acqrel) th0 th1)
+    :
+      (<<STEPS: rtc (SCThread.all_step L) th0 th1>>) \/
+      (exists th',
+          (<<STEPS0: rtc (SCThread.all_step L) th0 th'>>) /\
+          (<<STEPS1: rtc (OrdThread.all_step L Ordering.acqrel Ordering.acqrel) th' th1>>) /\
+          (<<RACE: SCRace.race L th'>>)).
+  Proof.
+    induction STEPS; eauto. dup H. inv H.
+    eapply ra_thread_step_sc_thread_step_or_race in USTEP; eauto. des.
+    - left. econs; eauto. econs; eauto.
+    - right. exists th'. esplits; eauto. econs; eauto. econs; eauto.
+    - right. exists x. esplits; eauto.
+    - right. exists x. esplits; eauto.
+  Qed.
+
+  Lemma ra_configuration_step_sc_configuration_step_or_race e tid c0 c1
+        (STEP: OrdConfiguration.estep L Ordering.acqrel Ordering.acqrel e tid c0 c1)
+        (WF: Configuration.wf c0)
+    :
+      (<<STEP: SCConfiguration.estep L e tid c0 c1>>) \/
+      (<<RACE: SCRace.race_steps L c0 tid>>).
+  Proof.
+    destruct (classic (SCRace.race_steps L c0 tid)) as [RACE|RACE]; auto. left.
+    inv STEP.
+
+    exploit ra_thread_step_sc_thread_step_or_race; try apply STEP0.
+    i. des; cycle 1.
+    { exfalso. eapply RACE. unfold SCRace.race_steps. esplits; eauto. }
+
+    econs; eauto.
+  Qed.
+
+  Lemma ra_configuration_steps_sc_configuration_steps_or_race c0 c1
+        (STEPS: rtc (OrdConfiguration.all_step L Ordering.acqrel Ordering.acqrel) c0 c1)
+        (WF: Configuration.wf c0)
+    :
+      (<<STEPS: rtc (SCConfiguration.all_step L) c0 c1>>) \/
+      (exists c' tid,
+          (<<STEPS: rtc (SCConfiguration.all_step L) c0 c'>>) /\
+          (<<RACE: SCRace.race_steps L c' tid>>)).
+  Proof.
+    ginduction STEPS; eauto. i. inv H.
+    eapply ra_configuration_step_sc_configuration_step_or_race in STEP; eauto. des.
+    { exploit SCConfiguration.estep_future; eauto. i. des.
+      exploit IHSTEPS; eauto. i. des.
+      { left. econs; eauto. econs; eauto. }
+      { right. esplits; [|eapply RACE]. econs; eauto. econs; eauto. }
+    }
+    { right. esplits; eauto. }
+  Qed.
+
+  Lemma ra_behavior_sc_behavior_or_race c
+        (RACEFREE: SCRace.racefree L c)
+        (WF: Configuration.wf c)
+    :
+      behaviors (@OrdConfiguration.step L Ordering.acqrel Ordering.acqrel) c <2=
+      behaviors (@SCConfiguration.step L) c.
+  Proof.
+    i. ginduction PR; eauto; i.
+    - econs 1; eauto.
+    - inv STEP.
+      eapply ra_configuration_step_sc_configuration_step_or_race in STEP0; eauto. des.
+      + econs 2; eauto.
+        * rewrite <- H0. econs; eauto.
+        * eapply IHPR; eauto.
+          { eapply SCRace.step_racefree; eauto. econs; eauto. }
+          { eapply SCConfiguration.step_future; eauto. econs; eauto. }
+      + exfalso. eapply RACEFREE; eauto.
+    - inv STEP.
+      eapply ra_configuration_step_sc_configuration_step_or_race in STEP0; eauto. des.
+      + econs 3; eauto.
+        * rewrite <- H0. econs; eauto.
+      + exfalso. eapply RACEFREE; eauto.
+    - inv STEP.
+      eapply ra_configuration_step_sc_configuration_step_or_race in STEP0; eauto. des.
+      + econs 4; eauto.
+        * rewrite <- H0. econs; eauto.
+        * eapply IHPR; eauto.
+          { eapply SCRace.step_racefree; eauto. econs; eauto. }
+          { eapply SCConfiguration.step_future; eauto. econs; eauto. }
+      + exfalso. eapply RACEFREE; eauto.
+    - econs 5.
+  Qed.
+
+  Lemma sc_racefree_ra_racefree c
+        (RACEFREE: SCRace.racefree L c)
+        (WF: Configuration.wf c)
+    :
+      RARace.racefree L c.
+  Proof.
+    ii. unfold RARace.race in *. des.
+    exploit ra_configuration_steps_sc_configuration_steps_or_race.
+    { etrans.
+      { eapply STEPS1. } econs 2.
+      { econs; eauto. }
+      { eapply STEPS2. }
+    }
+    { eauto. }
+    i. des.
+    2:{ eapply RACEFREE; eauto. }
+    inv RACE.
+    { des. eapply RACEFREE; [eauto|]. unfold SCRace.race_steps. esplits; eauto.
+      assert (exists from msg, (<<GET: Memory.get loc to c3.(Configuration.global).(Global.memory) = Some (from, msg)>>) /\ (<<NRESERVE: msg <> Message.reserve>>)).
+      { hexploit OrdConfiguration.rtc_all_step_future; [eapply STEPS1|..]; eauto.
+        i. des.
+        hexploit OrdConfiguration.estep_future; eauto. i. des.
+        hexploit OrdConfiguration.rtc_all_step_future; [eapply STEPS2|..]; eauto. i. des.
+        inv WRITE_STEP. ss.
+        hexploit OrdThread.step_future; eauto.
+        { eapply WF2; eauto. }
+        { eapply WF2. }
+        i. ss. des.
+        assert (exists from msg, (<<GET: Memory.get loc to gl2.(Global.memory) = Some (from, msg)>>) /\ (<<NRESERVE: msg <> Message.reserve>>)).
+        { inv STEP0. inv LOCAL; ss.
+          { clarify. inv LOCAL0. inv STEP0. esplits.
+            { eapply Memory.add_get0; eauto. }
+            { ss. }
+          }
+          { clarify. inv LOCAL2. inv STEP0. esplits.
+            { eapply Memory.add_get0; eauto. }
+            { ss. }
+          }
+        }
+        des. eapply Global.future_le in GL_FUTURE1. inv GL_FUTURE1.
+        destruct msg; ss. eapply MEMORY in GET. eauto.
+      }
+      des. unfold RARace.wr_race, SCRace.race in *. esplits; eauto.
+      { instantiate (1:=loc). destruct e; ss; clarify. }
+      { des; auto. }
+      econs. esplits; eauto. ss. des; auto.
+    }
+    { des. eapply RACEFREE; [eauto|]. unfold SCRace.race_steps. esplits; eauto.
+      assert (exists from msg, (<<GET: Memory.get loc to c3.(Configuration.global).(Global.memory) = Some (from, msg)>>) /\ (<<NRESERVE: msg <> Message.reserve>>)).
+      { hexploit OrdConfiguration.rtc_all_step_future; [eapply STEPS1|..]; eauto.
+        i. des.
+        hexploit OrdConfiguration.estep_future; eauto. i. des.
+        hexploit OrdConfiguration.rtc_all_step_future; [eapply STEPS2|..]; eauto. i. des.
+        inv WRITE_STEP. ss.
+        hexploit OrdThread.step_future; eauto.
+        { eapply WF2; eauto. }
+        { eapply WF2. }
+        i. ss. des.
+        assert (exists from msg, (<<GET: Memory.get loc to gl2.(Global.memory) = Some (from, msg)>>) /\ (<<NRESERVE: msg <> Message.reserve>>)).
+        { inv STEP0. inv LOCAL; ss.
+          { clarify. inv LOCAL0. inv STEP0. esplits.
+            { eapply Memory.add_get0; eauto. }
+            { ss. }
+          }
+          { clarify. inv LOCAL2. inv STEP0. esplits.
+            { eapply Memory.add_get0; eauto. }
+            { ss. }
+          }
+        }
+        des. eapply Global.future_le in GL_FUTURE1. inv GL_FUTURE1.
+        destruct msg; ss. eapply MEMORY in GET. eauto.
+      }
+      des. unfold RARace.ww_race, SCRace.race in *. esplits; eauto.
+      { instantiate (1:=loc). destruct e; ss; clarify. }
+      { des; auto. }
+      econs. esplits; eauto. ss. des; auto.
+    }
+  Qed.
+
+End SIM.
+
+
+(* LDRF-SC theorem *)
+Theorem local_drf_sc L
+        s
+        (RACEFREE: SCRace.racefree_syn L s):
+  behaviors (PFConfiguration.step ThreadEvent.get_machine_event_pf) (Configuration.init s) <2=
+  behaviors (@SCConfiguration.step L) (Configuration.init s).
+Proof.
+  i. eapply local_drf_ra in PR; eauto.
+  - eapply ra_behavior_sc_behavior_or_race; eauto.
+    eapply Configuration.init_wf; eauto.
+  - eapply sc_racefree_ra_racefree; eauto.
+    eapply Configuration.init_wf; eauto.
+Qed.
